theories/Reduction.v
@@ -1,5 +1,8 @@
-From MetaCoq.PCUIC Require Import PCUICAst PCUICAstUtils.
-From LogRel Require Import Automation Untyped DeclarativeTyping Generation Properties.
+From MetaCoq.PCUIC Require Import PCUICAst PCUICAstUtils PCUICRenameConv PCUICSigmaCalculus PCUICInstConv.
+From LogRel Require Import Notations Untyped Weakening GenericTyping DeclarativeTyping Properties Generation.
+
+#[local] Open Scope untagged_scope.
+Import DeclarativeTypingData.
 
 (** Inclusion of the various reduction-like *)
 
@@ -7,7 +10,10 @@ Definition RedConvTe {Γ} {t u A : term} :
     [Γ |- t ⇒ u : A] -> 
     [Γ |- t ≅ u : A].
 Proof.
-    induction 1 ; mltt.
+    induction 1.
+    1,3: now econstructor.
+    econstructor ; eauto.
+    now econstructor.
 Qed.
 
 Corollary termRedFrag Γ t u A : [Γ |- t ⇒ u : A] ->
@@ -15,42 +21,35 @@ fragment t && fragment u && fragment A && fragment_ctx Γ.
 Proof.
   intros.
   apply wfFrag.
-  mltt.
+  now eapply RedConvTe.
 Qed.
 
 Definition RedConvTeC {Γ} {t u A : term} :
     [Γ |- t ⇒* u : A] -> 
     [Γ |- t ≅ u : A].
 Proof.
-  induction 1 ; mltt.
+  induction 1.
+  1: now constructor.
+  eapply TermTrans ; tea.
+  now apply RedConvTe.
 Qed.
 
 Definition RedConvTy {Γ} {A B : term} :
     [Γ |- A ⇒ B] -> 
     [Γ |- A ≅ B].
 Proof.
-  induction 1 ; mltt.
+  destruct 1.
+  now (econstructor ; eapply RedConvTe ; eassumption).
 Qed.
 
 Definition RedConvTyC {Γ} {A B : term} :
     [Γ |- A ⇒* B] -> 
     [Γ |- A ≅ B].
 Proof.
-  induction 1 ; mltt.
-Qed.
-
-Definition TypeRedWFConv {Γ} {A B} :
-    [Γ |- A :⇒*: B] ->
-    [Γ |- A ≅ B].
-Proof.
-  intros [] ; mltt.
-Qed.
-
-Definition RedConvTeWFC {Γ} {t u A} :
-    [Γ |- t :⇒*: u : A] ->
-    [Γ |- t ≅ u : A].
-Proof.
-  intros [] ; mltt.
+  induction 1.
+  1: now econstructor.
+  eapply TypeTrans ; tea.
+  now apply RedConvTy.
 Qed.
 
 (** Whnf do not reduce *)
@@ -59,14 +58,7 @@ Lemma whne_nored Γ n u A :
   whne Γ n -> [Γ |- n ⇒ u : A] -> False.
 Proof.
   intros ne red.
-  induction red in ne |- *.
-  - inversion ne ; subst.
-    1: easy.
-    eapply mkApps_tApp_inj in H as [-> ->] ; cbn in *.
-    2: easy.
-    apply termRedFrag in red.
-    rewrite fragment_mkApps in red ; cbn in red.
-    now congruence.
+  induction red in ne |- * ; fold_decl.
   - inversion ne ; subst ; clear ne.
     1: now eapply neLambda.
     eapply mkApps_tApp_inj in H as [H ->] ; cbn in *.
@@ -75,6 +67,13 @@ Proof.
     apply mkApps_nisApp in H as [].
     2: cbn.
     all: congruence.
+  - inversion ne ; subst.
+    1: easy.
+    eapply mkApps_tApp_inj in H as [-> ->] ; cbn in *.
+    2: easy.
+    apply termRedFrag in red.
+    rewrite fragment_mkApps in red ; cbn in red.
+    now congruence.
   - easy.
 Qed.
 
@@ -83,18 +82,6 @@ Lemma whnf_nored Γ n u A :
 Proof.
   intros nf red.
   induction red in nf |- *.
-  - inversion nf ; subst.
-    2-5:
-      match goal with
-        | H : mkApps _ _ = tApp _ _ |- _ =>
-          apply mkApps_tApp_inj in H as [-> ->]
-      end ; [|easy] ;
-      apply termRedFrag in red ;
-      rewrite fragment_mkApps in red ; cbn in red ;
-      now congruence.
-    eapply whne_nored.
-    1: eassumption.
-    mltt.
   - inversion nf.
     2-5:
       match goal with
@@ -111,6 +98,18 @@ Proof.
     end ; [|easy] ;
     symmetry in He ;
     apply mkApps_nisApp in He as [] ; cbn ; congruence.
+  - inversion nf ; subst.
+    2-5:
+      match goal with
+        | H : mkApps _ _ = tApp _ _ |- _ =>
+          apply mkApps_tApp_inj in H as [-> ->]
+      end ; [|easy] ;
+      apply termRedFrag in red ;
+      rewrite fragment_mkApps in red ; cbn in red ;
+      now congruence.
+    eapply whne_nored.
+    1: eassumption.
+    now econstructor.
   - easy.
 Qed.
 
@@ -131,19 +130,19 @@ Proof.
   induction red in v, B, red' |- *.
   - eapply termRedGen in red' as [? [d]].
     inversion d ; subst ; clear d.
+    + exfalso.
+      eapply whnf_nored.
+      2: eassumption.
+      now econstructor.
+    + reflexivity.
+  - eapply termRedGen in red' as [? [d]].
+    inversion d ; subst ; clear d.
     + f_equal.
       eauto.
     + exfalso.
       eapply whnf_nored.
       2: eassumption.
       now econstructor.
-  - eapply termRedGen in red' as [? [d]].
-    inversion d ; subst ; clear d.
-    + exfalso.
-      eapply whnf_nored.
-      2: eassumption.
-      now econstructor.
-    + reflexivity.
   - easy.
 Qed.
 
@@ -155,3 +154,143 @@ Proof.
   destruct HB, HB'.
   now eapply red_det.
 Qed.
+
+
+Lemma redtm_wk {Γ Δ t u A} (ρ : Δ ≤ Γ) :
+[|- Δ ] -> [Γ |- t ⇒ u : A] -> [Δ |- t.[ren ρ] ⇒ u.[ren ρ] : A.[ren ρ]].
+Proof.
+  intros ? red.
+  induction red as [? ? ? ? ? ? Ht Ha | |]; fold_decl.
+  - cbn in *.
+    rewrite ! subst10_inst.
+    eapply redtm_meta_conv.
+    1: econstructor ; fold_decl.
+    1,3: now eapply typing_wk.
+    + unshelve eapply typing_wk in Ht.
+      3: econstructor ; now eapply well_lift.
+      1: shelve.
+      2: now econstructor ; [eassumption | eapply typing_wk].
+      cbn in *.
+      now replace (t.[_]) with (t.[ren (wk_lift ρ)])
+        by (cbn ; now rewrite ren_shiftn).
+    + cbn.
+      now rewrite <- up_Up, ren_shiftn.
+    + now rewrite <- up_Up, ren_shiftn.
+  - cbn in *.
+    rewrite subst10_inst.
+    econstructor ; fold_decl.
+    2: now eapply typing_wk.
+    eapply redtm_meta_conv ; try easy.
+    f_equal.
+    now rewrite up_Up.
+  - econstructor.
+    1: eassumption.
+    now eapply typing_wk.
+Qed.
+
+Lemma redty_wk {Γ Δ A B} (ρ : Δ ≤ Γ) :
+[|- Δ ] -> [Γ |- A ⇒ B] -> [Δ |- A.[ren ρ] ⇒ B.[ren ρ]].
+Proof.
+  intros ? red.
+  destruct red.
+  constructor.
+  fold_decl.
+  change U with (U.[ren ρ]).
+  now apply redtm_wk.
+Qed.
+
+Module DeclarativeConvProp.
+
+  #[export, refine] Instance ConvTypeDeclProp : ConvTypeProp (ta := de) := {}.
+  Proof.
+  - now econstructor.
+  - intros.
+    constructor ; red ; intros.
+    all: now econstructor.
+  - intros.
+    now apply typing_wk.
+  - intros.
+    eapply TypeTrans ; [eapply TypeTrans | ..].
+    2: eassumption.
+    2: eapply TypeSym.
+    all: now eapply RedConvTyC.
+  - econstructor.
+    now econstructor.
+  - now econstructor.
+  Qed.
+
+  #[export, refine] Instance ConvTermDeclProp : ConvTermProp (ta := de) := {}.
+  Proof.
+  - intros.
+    constructor ; red ; intros.
+    all: now econstructor.
+  - intros.
+    now econstructor.
+  - intros.
+    now eapply typing_wk.
+  - intros.
+    eapply TermConv.
+    2: now eapply TypeSym, RedConvTyC.
+    eapply TermTrans ; [eapply TermTrans |..].
+    2: eassumption.
+    2: eapply TermSym.
+    all: now eapply RedConvTeC.
+  - eauto.
+  - intros.
+    now econstructor.
+  - intros.
+    now econstructor.
+  Qed.
+
+  #[export, refine] Instance ConvNeuDeclProp : ConvNeuProp (ta := de) := {}.
+  Proof.
+  - split ; red ; intros.
+    all: now econstructor.
+  - intros.
+    now eapply TermConv.
+  - intros.
+    now eapply typing_wk.
+  - intros.
+    now econstructor.
+  - intros.
+    now econstructor.
+  Qed.
+  
+  #[export, refine] Instance OneRedTermDeclProp : OneRedTermProp (ta := de) := {}.
+  Proof.
+  - intros.
+    now eapply redtm_wk.
+  - intros.
+    eapply whnf_nored ; eassumption.
+  - intros.
+    now eapply red_det.
+  - intros.
+    now econstructor.
+  - intros.
+    now econstructor.
+  - intros.
+    now econstructor.
+  Qed. 
+
+  #[export, refine] Instance OneRedTypeDeclProp : OneRedTypeProp (ta := de) := {}.
+  Proof.
+  - intros.
+    now eapply redty_wk.
+  - intros.
+    now eapply whnf_nored_ty.
+  - intros.
+    now eapply red_det_ty.
+  - intros.
+    now econstructor.
+  Qed.
+
+End DeclarativeConvProp.
+
+Module DeclarativeTypingProp.
+  Import DeclarativeTypingData DeclarativeTypingProp DeclarativeConvProp.
+
+  #[export] Instance DeclarativeTypingProp : GenericTypingProp de _ _ _ _ _ _ _ _ := {}.
+
+End DeclarativeTypingProp.
+
+Import DeclarativeTypingProp.
