theories/Utils.v
@@ -1,6 +1,0 @@
-From MetaCoq Require Import utils.
-
-Definition iff (A B : Type) :=
-  (A -> B) × (B -> A).
-
-Notation "A <-> B" := (iff A B) : type_scope.
